ber_fetch_length exec on int; proof until loop [skip ci]

src/Lib/BCT/BFL/Vst.v
@@ -1,43 +1,148 @@
 Require Import Core.Core Core.StructNormalizer VstLib.
 Require Import VST.floyd.proofauto.
-Require Import BFL.Exec.
+(* Require Import BFL.Exec. *)
 Require Import Clight.ber_tlv_length.
+Require Import Core.Notations Core.SepLemmas Core.Tactics Core.VstTactics.
 
 Instance CompSpecs : compspecs. Proof. make_compspecs prog. Defined.
 Definition Vprog : varspecs. Proof. mk_varspecs prog. Defined.
 
 Section Ber_fetch_len.
 
+Open Scope  bool.
+Open Scope int.
+Fixpoint aux_loop ptr len skip oct size sizeofval :
+   (int * int * int * int) := 
+  match ptr with
+  | x :: xs => if (negb (oct == 0)) && ((skip + 1) <=u size)
+              then if (len >> ((Int.repr 8 * sizeofval) - (Int.repr 8 + 1))) == 0
+                   then let len' := Int.or (len << Int.repr 8) x in
+                        aux_loop xs len' (skip + 1) (oct - 1) size sizeofval
+                   else (Int.neg 1, oct, len, skip)
+              else (0, oct, len, skip)
+  | nil => (0, 0, 0, 0)
+  end.
+
+Definition bfl_loop ptr len  skip oct size sizeofval
+  := aux_loop ptr len skip oct size sizeofval.
+
+
+Definition ber_fetch_len ptr isc len_r size sizeofval rssizem : 
+   (int * int) :=
+  if eq_dec size 0
+  then (0, len_r)
+  else let oct := Znth 0 ptr in 
+       if eq_dec (oct & Int.repr 128) 0
+       then (1, oct)
+       else if (negb (isc =? 0)) && (oct == Int.repr 128) 
+            then (1, Int.neg 1)
+            else if eq_dec oct (Int.repr 255)
+                 then (Int.neg 1, len_r)
+                 else let oct := oct & (Int.repr 127) in
+                      match bfl_loop (skipn 1%nat ptr) 0 1 oct size sizeofval with
+                      | (z, oct, len, skip) => if eq_dec z (Int.neg 1) 
+                                       then (z, len_r)
+                                       else 
+                                         if eq_dec oct 0 
+                                              then if (len < 0) || (rssizem < len)
+                                                   then (Int.neg 1, len_r)
+                                                   else (skip, len)
+                                              else (0, len_r)
+                      end.
+
+Open Scope Z.
+
 Definition ber_fetch_len_spec : ident * funspec :=
   DECLARE _ber_fetch_length
-    WITH c : Z,  buf_p : val,
-         size : Z, data : list Z,
-         res_ptr : val
+    WITH c : Z,  b : block, i : ptrofs,
+         size : int, data : list int,
+         len_r : val
     PRE [tint, tptr tvoid, tuint, tptr tint]
       PROP ((* isptr buf_p; *)
-            (* isptr res_ptr;
-               Zlength data = size; *)
-            0 <= size <= Int.max_unsigned)
-      PARAMS (Vint (Int.repr c); buf_p; Vint (Int.repr size); res_ptr)
+            (* isptr len_r;
+            Zlength data = size; *)
+        c = 0;
+        Ptrofs.unsigned i + len data < Ptrofs.modulus;
+        Forall (fun x => 0 <= Int.unsigned x <= Byte.max_unsigned) data;
+            0 < len data)
+      PARAMS (Vint (Int.repr 0); (Vptr b i); Vint size; len_r)
       GLOBALS ()
       SEP (data_at Tsh (tarray tuchar (Zlength data)) 
-                   (map Vubyte (map Byte.repr data)) buf_p;
-           data_at_ Tsh tint res_ptr)
+                   (map Vint data) (Vptr b i);
+           data_at_ Tsh tint len_r)
     POST [tint]
-      let r := ber_fetch_len data c 0 size (sizeof tuint) Int.modulus in
+      let r := ber_fetch_len data c 0%int size (Int.repr (sizeof tuint))
+       (Int.repr (Int.max_unsigned)) in
       PROP ()
-      LOCAL (temp ret_temp (Vint (Int.repr (fst r))))
+      LOCAL (temp ret_temp (Vint ((fst r))))
       SEP (data_at Tsh (tarray tuchar (Zlength data)) 
-                   (map Vubyte (map Byte.repr data)) buf_p;
-           data_at Tsh tint (Vubyte (Byte.repr (snd r))) res_ptr).
+                   (map Vint (data)) (Vptr b i);
+           if eq_dec (fst r) 0%int                     
+           then  data_at_ Tsh tint len_r
+           else if eq_dec (fst r) (Int.neg 1%int)
+                then  data_at_ Tsh tint len_r
+                else 
+                  data_at Tsh tint (Vint (snd r)) len_r).
 
 Definition Gprog := ltac:(with_library prog [ber_fetch_len_spec]).
 
-Theorem ber_fetch_len : semax_body Vprog Gprog 
+Theorem ber_fetch_len_corr : semax_body Vprog Gprog 
                                           (normalize_function f_ber_fetch_length
                                                               composites) 
                                           ber_fetch_len_spec.
 Proof.
+start_function.
+forward.
+forward_if.
+forward.
+erewrite split_non_empty_list 
+  with (i := Vint (Znth 0 data)) 
+       (j2 := len data - 1) 
+       (ls' := sublist 1 (len data) (map Vint data)).
+Intros.
+forward.
+admit. (*entailer!.
+eapply Forall_Znth with (i0 := 0) in H; try lia.
+strip_repr. *)
+forward_if.
+- admit.
+ (* forward.
+  forward.
+  unfold ber_fetch_len.
+  repeat rewrite_if_b.
+  simpl.
+  erewrite <- split_non_empty_list
+    with (i := Vint (Znth 0 data))
+         
+         (ls' := sublist 1 (len data) (map Vint data)).
+  entailer!.
+  erewrite <- map_sublist.
+  erewrite <- map_cons.
+  f_equal.
+  assert (Znth_0_cons_sublist :  forall (ls : list int), 
+             0 < len ls ->
+             Znth 0 ls :: sublist 1 (len ls) ls = ls).
+  { intros.
+    erewrite Znth_cons_sublist.
+    autorewrite with sublist.
+    auto. lia. }
+  erewrite Znth_0_cons_sublist; auto; try lia.
+  1-2: autorewrite with sublist; rep_omega.
+  auto. *)
+- forward_if (temp _t'1 Vzero); try contradiction.
+  + admit.
+    (* forward.
+       entailer!. *)
+  + forward_if; try contradiction.
+    forward_if.
+    * admit. (* forward.
+      { unfold ber_fetch_len.
+        repeat rewrite_if_b.
+        simpl.
+        entailer!.
+        admit. (* split as before *) } *)
+    * repeat forward.
+      (* Loop *)
 Admitted.
 
 End Ber_fetch_len.
